NuSys.thy
@@ -4,7 +4,7 @@ theory NuSys
   imports NuPrim NuLLReps
   keywords
     "proc" :: thy_goal_stmt
-  and "as" "\<rightarrow>" "\<longmapsto>" "\<leftarrow>" "^" "^*" "cast" :: quasi_command
+  and "as" "\<rightarrow>" "\<longmapsto>" "\<leftarrow>" "^" "^*" "cast" "requires" :: quasi_command
   and "\<bullet>" "affirm" "\<nu>have" "\<nu>obtain" "\<nu>choose" "\<medium_left_bracket>" "\<medium_right_bracket>" "reg" "\<Longrightarrow>" "drop_fact" "\<nu>debug" :: prf_decl % "proof"
   and "\<nu>processor" "\<nu>processor_resolver" "\<nu>exty_simproc" :: thy_decl % "ML"
   and "\<nu>overloads" "\<nu>cast_overloads" :: thy_decl
@@ -71,10 +71,11 @@ in
 val _ = Outer_Syntax.local_theory \<^command_keyword>\<open>\<nu>exty_simproc\<close> "setup the pecific simproc for \<^const>\<open>ExTy\<close>"
   (Parse.binding >> NuExTyp.set_simproc_cmd)
 
+val requires_statement = Scan.optional (Parse.$$$ "requires" |-- Parse.!!! Parse_Spec.statement) [];
 val _ =
   Outer_Syntax.local_theory_to_proof' \<^command_keyword>\<open>proc\<close> "begin a procedure construction"
     ((Parse_Spec.thm_name ":" -- Parse.term --| $$$ "\<longmapsto>" -- Parse.term -- Parse.for_fixes -- Scan.optional Parse_Spec.includes []
-            -- Parse_Spec.if_statement) >>
+            -- requires_statement) >>
         (fn (((((b,arg),ret),fixes),includes),preconds) =>  
             (begin_proc_cmd b arg ret fixes includes preconds)));
 
